---
title: "1+2 = 3, 4+5+6 = 7+8"
format:
  html:
    toc: true
    # toc-location: left
    toc-title: " "
author: "Mog Man"
date: "2023-11-27"
categories: false
image: "image2.png"
---

### Problem

The following elegant pattern is observed:

 

```{=tex}
\begin{align}
1+2&=3 \\
4+5+6 &=7+8 \\
9+10+11+12&=13+14+15 \\
16+17+18+19+20&=21+22+23+24 \\
25+26+27+28+29+30&=31+32+33+34+35 \\
36+37+38+39+40+41+42&=43+44+45+46+47+48 \\
\end{align}
```
 

Each line is formed by counting up the natural numbers , continuing the count of the previous line. Starting at $[1+2=3]$, each side of the equation has one more term than the previous line.

Why does this pattern occur and does it continue on forever?

### Solution

The first observation we can make is that each line begins with a square number. Do all equations in this format begin with a square number on the left side?

For a generic equation in this format: $A + (x+1) + (x+2) + \cdots (x+n) = (x+n+1) +(x+n+2) + \cdots (x +2n)$

we find that each term after $A$ on the left hand side of the equation is $n$ smaller than a corresponding term on the right hand side. Given there are $n$ of these terms it follows that $A$ must be $n^2$

The length of each line of the pattern can be expressed as $2n + 1$ Given it counts up sequentially, the first number of each line is equal to the sum of all previous line lengths, $+1$:

```{=tex}
\begin{align}
1 +\sum_{k=1}^{n-1} (2k+1) 
\end{align}
```
This can be rearranged as so:

```{=tex}
\begin{align}
1 -(2n +1) +&\sum_{k=1}^{n} (2k+1) \\
=-2n +n +&\sum_{k=1}^{n} 2k \\
= -n + 2 \cdot&\sum_{k=1}^{n} k
\end{align}
```
Given: \begin{align}
\sum_{k=1}^{n} k = \frac{n(n+1)}{2}
\end{align}

```{=tex}
\begin{align}
&n + 2(\frac{n(n+1)}{2}) \\
=-&n +n^2 +n \\
= \space \space \space &n^2
\end{align}
```
$(n-1)^2,\  n^2,\  (n+1)^2$ depicts a generic sequence of squares. let $a$ be the difference between $n^2$ and $(n-1)^2$ and $b$ be the difference between $n^2$ and $(n+1)^2$

If this is true, we should expect that the difference between $a$ and $b$ to be $2$.

In equation format:

```{=tex}
\begin{align}
(n-1)^2 = n^2 + a = (n+1)^2 +a +b\\
\end{align}
```
thus:

```{=tex}
\begin{align}
a &= (n-1)^2 - n^2 \\
&= n^2 - 2n +1 - n^2 \\
&= - 2n +1 \\
\end{align}
```
```{=tex}
\begin{align}
b &= n^2 +a - ((n+1)^2 +a)\\
&= n^2 +a -(n^2 +2n +1 +a) \\
&= n^2 +a -n^2 -2n -1 -a) \\
&= - 2n -1 \\
\end{align}
```
```{=tex}
\begin{align}
a - b &= -2n +1 - (-2n-1) \\
&= -2n +1 +2n +1 \\
&= 2 \\
\end{align}
```
Thus the difference of the difference between adjacent squares is $2$

The general formula for any line $n$ where line $n=1$ is $1+2 =3$:

```{=tex}
\begin{align}
n^2 + (n^2+1) + (n^2+2) + \cdots (n^2+n) = (n^2+n+1)  + \cdots (n^2 +2n)
\end{align}
```
```{=tex}
\begin{align}
 \sum_{i=0}^n (n^2 +i) =  \sum_{i=1}^n (n^2 +n+i)
\end{align}
```

------------------------------------------------------------------------

### Cubic sequence

As I was exploring the pattern to work out a proof, I stumbled upon the fact that the difference of the difference of the difference of the value of each line was constant.

The first line is made up of values of lines between $n=1$ and $n=7$. Each subsequent line is made up by taking the difference between the adjacent terms of the previous line $$3\qquad 15 \qquad 42 \qquad 90 \qquad 165\qquad 273\qquad 420$$ $$12\qquad 27\qquad 48\qquad 75\qquad 108\qquad 147$$ $$15\qquad 21 \qquad 27 \qquad 33\qquad 39$$ $$6 \qquad 6 \qquad 6 \qquad 6 $$

Polynomials of the degree $n$ have a constant non-zero $n^{th}$ difference, so the $3^{rd}$ difference being constant $6$ here is indicative of a cubic polynomial.

Finding the formula for this sequence is a straightforward process of symultaneous equations, generated by using the general format of a cubic \[$an^3 + bn^2 + cn + d$\] and equating it to the first four values in the sequence:

```{=tex}
\begin{align}
1: \quad&a + b + c + d = 3 \\
2: \quad&8a + 4b + 2c + d = 15 \\
3: \quad&27a + 9b + 3c + d = 42 \\
4: \quad&64a + 16b + 4c + d = 90 \\
\end{align}
```
Taking equation $1$ from $2$ we eliminate $d$: \begin{align}
5: \quad&7a +3b +c = 12\\
\end{align}

Taking eq. $2$ from $3$:

```{=tex}
\begin{align}
6: \quad&19a +5b +c = 27\\
\end{align}
```
Taking eq. $3$ from $4$:

```{=tex}
\begin{align}
7: \quad&37a +7b +c = 48\\
\end{align}
```
Taking eq. $5$ from $6$ and eliminating $c$:

```{=tex}
\begin{align}
8: \quad&12a +2b = 15\\
\end{align}
```
Taking eq. $6$ from $7$:

```{=tex}
\begin{align}
9: \quad&18a +2b = 21\\
\end{align}
```
Taking eq. $8$ from $9$ and eliminating $b$ we get: \begin{align}
6a &= 6 \\
a &= 1
\end{align}

Substituting $a = 1$ into eq. $8$ we get \begin{align}
12 +2b &= 15 \\
2b &= 3 \\
b &= \frac{3}{2}
\end{align}

Substituting $a = 1$ and $b = \frac{3}{2}$ into eq. $5$ we get: \begin{align}
7 + \frac{9}{2}+c &= 12\\
c &= \frac{24}{2} - \frac{23}{2} \\
c &= \frac{1}{2}
\end{align}

Substituting $a = 1$, $b = \frac{3}{2}$ and $c = \frac{1}{2}$ into eq. $1$ we get:

```{=tex}
\begin{align}
d &= 3 - 1 -\frac{3}{2} - \frac{1}{2} \\
d &= 0
\end{align}
```
Thus our formula for the $n^{th}$ term is: \begin{align}
n^3 + \frac{3n^2}{2} + \frac{n}{2} \\
\end{align}

#### Where does this cubic come from?

We already determined that each line is given as: \begin{align}
\sum_{i=0}^n (n^2 +i) =  \sum_{i=1}^n (n^2 +n+i)
\end{align}

Taking the right side of the equation, it can be rearranged as so:

```{=tex}
\begin{align}
\sum_{i=1}^n (n^2 +n+i) \\
= n^3 + n^2 + \sum_{i=1}^n (i) \\
\end{align}
```
Given: \begin{align}
\sum_{k=1}^{n} k = \frac{n(n+1)}{2}
\end{align}

```{=tex}
\begin{align}
&n^3 + n^2 +(\frac{n(n+1)}{2}) \\
= &n^3 + n^2 +\frac{n^2 + n}{2} \\
=&n^3 + \frac{3n^2}{2} + \frac{n}{2} 
\end{align}
```